Define a typeclass for Atoms. Provide implementations for the concrete Atom type and for natural numbers. Define the LocallyNameless class and attach the notations to it. Provide an implementation for STLC terms. Automate most proofs using decide with a custom tactic.

LocallyNameless/STLC.v
@@ -4,76 +4,17 @@ Require Import
 
 Import ListNotations.
 
-(*
-Parameters
-  (Atom : Type)
-  (Decidable_eq_Atom : forall x y : Atom, Decidable (x = y))
-  (fresh : list Atom -> Atom)
-  (fresh_spec : forall l : list Atom, ~ In (fresh l) l).
+From FormalSystems Require Import LocallyNameless.LocallyNameless.
 
-Existing Instance Decidable_eq_Atom.
-*)
+(* From FormalSystems Require Import LocallyNameless.Atom. *)
 
-Inductive Atom : Type :=
-| fresh : list Atom -> Atom.
+Arguments decide : simpl never.
 
-Fixpoint size (x : Atom) : nat :=
-match x with
-| fresh l => 1 + fold_right (fun h t => size h + t) 0 l
+Ltac decide_all :=
+repeat match goal with
+| |- context [decide (?x = ?x)] => rewrite Decidable_complete by easy
+| |- context [decide (?x = ?y)] => decide (x = y); subst; cbn; try easy
 end.
-
-Definition sizes l := 1 + fold_right (fun h t => size h + t) 0 l.
-
-Require Import Lia.
-
-Lemma In_size :
-  forall (x : Atom) (l : list Atom),
-    In x l -> size x < sizes l.
-Proof.
-  induction l as [| h t IH]; intros Hin; [easy |].
-  destruct Hin as [-> | Hin]; cbn; [now lia |].
-  unfold sizes in IH.
-  specialize (IH Hin).
-  now lia.
-Qed.
-
-Lemma fresh_spec :
-  forall l : list Atom,
-    ~ In (fresh l) l.
-Proof.
-  intros l Hin.
-  apply In_size in Hin. cbn in Hin.
-  now lia.
-Qed.
-
-Fixpoint eq_dec_Atom (x y : Atom) : {x = y} + {x <> y}.
-Proof.
-  refine
-  (
-    match x, y with
-    | fresh lx, fresh ly =>
-      match list_eq_dec eq_dec_Atom lx ly with
-      | left eq => _
-      | right neq => _
-      end
-    end
-  ).
-  - now left; f_equal.
-  - now right; intros [=].
-Defined.
-
-#[export, refine] Instance Decidable_eq_Atom :
-  forall x y : Atom, Decidable (x = y) :=
-{
-  Decidable_witness :=
-    match eq_dec_Atom x y with
-    | left _ => true
-    | right _ => false
-    end;
-}.
-Proof.
-  now destruct (eq_dec_Atom x y).
-Qed.
 
 Inductive Ty : Type :=
 | TyUnit : Ty
@@ -134,8 +75,6 @@ end.
 
 Notation "x |> f" := (f x) (at level 68, only parsing).
 
-(* Notation "t [ x ~> u ]" := (subst x u t) (at level 68). *)
-
 Notation "t [[ x := u ]]" := (subst x u t) (at level 68).
 
 Lemma subst_demo :
@@ -179,186 +118,85 @@ Proof.
     now destruct IHt1, IHt2; firstorder congruence.
 Qed.
 
-Fixpoint open (i : nat) (u t : Tm) : Tm :=
+Fixpoint open (t : Tm) (i : nat) (u : Tm) : Tm :=
 match t with
 | fvar a    => fvar a
 | bvar j    => if decide (i = j) then u else bvar j
-| abs t'    => abs (open (S i) u t')
-| app t1 t2 => app (open i u t1) (open i u t2)
+| abs t'    => abs (open t' (S i) u)
+| app t1 t2 => app (open t1 i u) (open t2 i u)
 end.
 
-(* Notation "{ n ~> t2 } t1" := (open t1 n t2) (at level 68). *)
-Notation "t {{ i ~> u }}" := (open i u t) (at level 68).
+Notation "t {{ i ~> u }}" := (open t i u) (at level 68).
 
-Definition open' (u t : Tm) : Tm :=
-  open 0 u t.
+Fixpoint close (t : Tm) (i : nat) (a : Atom) : Tm :=
+match t with
+| fvar x    => if decide (a = x) then bvar i else fvar x
+| bvar n    => bvar n
+| abs t'    => abs (close t' (S i) a)
+| app t1 t2 => app (close t1 i a) (close t2 i a)
+end.
+
+Notation "t {{ i <~ a }}" := (close t i a) (at level 68).
 
 Lemma open_demo :
   forall y : Atom,
-    app (abs (app 1 0)) 0 |> open' y = app (abs (app y 0)) y.
+    app (abs (app 1 0)) 0 {{ 0 ~> y }} = app (abs (app y 0)) y.
 Proof.
   easy.
 Qed.
 
-(*
-Fixpoint close (a : Atom) (u t : Tm) : Tm :=
-match t with
-| fvar x    => if decide (a = x) then u else fvar x
-| bvar i    => bvar i
-| abs t'    => abs (close a (succ u) t')
-| app t1 t2 => app (close a u t1) (close a u t2)
-end.
+#[export] Instance OC_Tm : OC nat Atom Tm :=
+{
+  open := open;
+  close := close;
+}.
 
-Notation "t {{ u <~ a }}" := (close a u t) (at level 68).
-*)
-
-Fixpoint close (a : Atom) (i : nat) (t : Tm) : Tm :=
-match t with
-| fvar x    => if decide (a = x) then bvar i else fvar x
-| bvar n    => bvar n
-| abs t'    => abs (close a (S i) t')
-| app t1 t2 => app (close a i t1) (close a i t2)
-end.
-
-Notation "t {{ i <~ a }}" := (close a i t) (at level 68).
-
-(* OC 1 *)
-Lemma open_open_eq :
-  forall (t : Tm) (i : nat) (a b : Atom),
-    t {{ i ~> a }} {{ i ~> b }} = t {{ i ~> a }}.
+#[export, refine] Instance LocallyNameless_Tm : LocallyNameless nat Atom Tm := {}.
 Proof.
-  induction t; cbn; intros; [easy | | |].
-  - destruct (PeanoNat.Nat.eqb_spec i n); cbn; [easy |].
-    now destruct (PeanoNat.Nat.eqb_spec i n).
-  - now rewrite IHt.
-  - now rewrite IHt1, IHt2.
-Qed.
-
-(* OC 2 *)
-Lemma close_close_eq :
-  forall (t : Tm) (a : Atom) (i j : nat),
-    t {{ i <~ a }} {{ j <~ a }} = t {{ i <~ a }}.
-Proof.
-  induction t; cbn; intros; [| easy | |].
-  - decide (a0 = a); cbn; [easy |].
-    now decide (a0 = a).
-  - now rewrite IHt.
-  - now rewrite IHt1, IHt2.
-Qed.
-
-(* OC 3 *)
-Lemma open_close_eq :
-  forall (t : Tm) (i : nat) (a : Atom),
-    t {{ i ~> a }} {{ i <~ a }} = t {{ i <~ a }}.
-Proof.
-  induction t; cbn; intros; [easy | ..].
-  - destruct (PeanoNat.Nat.eqb_spec i n); subst; cbn; [| easy].
-    now decide (a = a).
-  - now rewrite IHt.
-  - now rewrite IHt1, IHt2.
-Qed.
-
-(* OC 4 *)
-Lemma close_open_eq :
-  forall (t : Tm) (i : nat) (a : Atom),
-    t {{ i <~ a }} {{ i ~> a }} = t {{ i ~> a }}.
-Proof.
-  induction t; cbn; intros; [| easy | ..].
-  - decide (a0 = a); subst; cbn; [| easy].
-    now destruct (PeanoNat.Nat.eqb_spec i i).
-  - now rewrite IHt.
-  - now rewrite IHt1, IHt2.
-Qed.
-
-(* OC 5 *)
-Lemma open_open_neq :
-  forall (t : Tm) (i j : nat) (a b : Atom),
-    i <> j ->
-      t {{ i ~> a }} {{ j ~> b }} = t {{ j ~> b }} {{ i ~> a }}.
-Proof.
-  induction t; cbn; intros; [easy | ..].
-  - destruct (PeanoNat.Nat.eqb_spec j n); cbn;
-      destruct (PeanoNat.Nat.eqb_spec i n); subst; cbn; [easy | | easy |].
-    + now destruct (PeanoNat.Nat.eqb_spec n n).
-    + now destruct (PeanoNat.Nat.eqb_spec j n).
-  - now rewrite IHt; [| congruence].
-  - now rewrite IHt1, IHt2.
-Qed.
-
-(* OC 6 *)
-Lemma close_close_neq :
-  forall (t : Tm) (i j : nat) (a b : Atom),
-    a <> b ->
-      t {{ i <~ a }} {{ j <~ b }} = t {{ j <~ b }} {{ i <~ a }}.
-Proof.
-  induction t; cbn; intros; [| easy | ..].
-  - decide (a0 = a); subst; cbn;
-      decide (b = a); subst; cbn; only 1, 3: easy.
-    + now decide (a = a).
-    + now decide (a0 = a).
-  - now rewrite IHt; [| congruence].
-  - now rewrite IHt1, IHt2.
-Qed.
-
-(* OC 7 *)
-Lemma open_close_neq :
-  forall (t : Tm) (i j : nat) (a b : Atom),
-    i <> j -> a <> b ->
-      t {{ i ~> a }} {{ j <~ b }} = t {{ j <~ b }} {{ i ~> a }}.
-Proof.
-  induction t; cbn; intros.
-  - decide (b = a); subst; cbn; [| easy].
-    now destruct (PeanoNat.Nat.eqb_spec i j).
-  - destruct (PeanoNat.Nat.eqb_spec i n); cbn; [| easy].
-    now decide (b = a); subst.
-  - now rewrite IHt; congruence.
-  - now rewrite IHt1, IHt2.
-Qed.
-
-(* OC 8 *)
-Lemma open_close_open :
-  forall (t : Tm) (i j : nat) (a b : Atom),
-    t {{ i ~> a }} {{ j <~ a }} {{ j ~> b }}
-      =
-    t {{ j ~> b }} {{ i <~ a }} {{ i ~> b }}.
-Proof.
-  induction t; cbn; intros.
-  - decide (a0 = a); cbn; [| easy].
-    now destruct (PeanoNat.Nat.eqb_spec j j), (PeanoNat.Nat.eqb_spec i i).
-  - destruct (PeanoNat.Nat.eqb_spec i n); subst; cbn;
-      destruct (PeanoNat.Nat.eqb_spec j n); subst; cbn.
-    + rewrite Decidable_complete by easy.
-      now decide (a = b); cbn; destruct (PeanoNat.Nat.eqb_spec n n).
-    + rewrite Decidable_complete by easy; cbn.
-      now destruct (PeanoNat.Nat.eqb_spec j j), (PeanoNat.Nat.eqb_spec n n).
-    + decide (a = b); cbn; [| easy].
-      now destruct (PeanoNat.Nat.eqb_spec i i).
-    + now destruct (PeanoNat.Nat.eqb_spec i n).
-  - now rewrite IHt.
-  - now rewrite IHt1, IHt2.
-Qed.
-
-(* OC 9 *)
-Lemma close_open_close :
-  forall (t : Tm) (i j : nat) (a b : Atom),
-    t {{ i <~ a }} {{ i ~> b }} {{ j <~ b }}
-      =
-    t {{ j <~ b }} {{ i ~> a }} {{ j <~ a }}.
-Proof.
-  induction t; cbn; intros.
-  - decide (b = a); subst; cbn; decide (a0 = a); subst; cbn.
-    + now destruct (PeanoNat.Nat.eqb_spec i j), (PeanoNat.Nat.eqb_spec i i); cbn;
-        rewrite ?Decidable_complete by easy.
-    + rewrite Decidable_complete by easy.
-      destruct (PeanoNat.Nat.eqb_spec i j); cbn; [| easy].
-      now rewrite Decidable_complete.
-    + destruct (PeanoNat.Nat.eqb_spec i i); cbn; [| easy].
-      now rewrite Decidable_complete.
-    + now decide (b = a).
-  - destruct (PeanoNat.Nat.eqb_spec i n); subst; cbn; [| easy].
-    now rewrite !Decidable_complete.
-  - now rewrite IHt.
-  - now rewrite IHt1, IHt2.
+  all: cbn.
+  - induction t; cbn; intros; [easy | | |].
+    + now decide_all.
+    + now rewrite IHt.
+    + now rewrite IHt1, IHt2.
+  - induction t; cbn; intros; [| easy | |].
+    + now decide_all.
+    + now rewrite IHt.
+    + now rewrite IHt1, IHt2.
+  - induction t; cbn; intros; [easy | ..].
+    + now decide_all.
+    + now rewrite IHt.
+    + now rewrite IHt1, IHt2.
+  - induction t; cbn; intros; [| easy | ..].
+    + now decide_all.
+    + now rewrite IHt.
+    + now rewrite IHt1, IHt2.
+  - induction t; cbn; intros; [easy | ..].
+    + now decide_all.
+    + now rewrite IHt; [| congruence].
+    + now rewrite IHt1, IHt2.
+  - induction t; cbn; intros; [| easy | ..].
+    + now decide_all.
+    + now rewrite IHt; [| congruence].
+    + now rewrite IHt1, IHt2.
+  - induction t; cbn; intros.
+    + now decide_all.
+    + now decide_all.
+    + now rewrite IHt; congruence.
+    + now rewrite IHt1, IHt2.
+  - induction t; cbn; intros.
+    + now decide_all.
+    + now decide_all.
+    + now rewrite IHt.
+    + now rewrite IHt1, IHt2.
+  - induction t; cbn; intros.
+    + now decide_all.
+    + now decide_all.
+    + now rewrite IHt.
+    + now rewrite IHt1, IHt2.
+Restart.
+  all: cbn;
+    (induction t; cbn; intros;
+      [now decide_all | now decide_all | now rewrite IHt; congruence | now rewrite IHt1, IHt2]).
 Qed.
 
 Lemma open_from_subst :
@@ -368,8 +206,7 @@ Lemma open_from_subst :
 Proof.
   induction t; cbn; intros.
   - now decide (a0 = a); subst; firstorder.
-  - destruct (PeanoNat.Nat.eqb_spec i n); cbn; [| easy].
-    now decide (a = a).
+  - now decide_all.
   - now rewrite <- IHt.
   - rewrite in_app_iff in H.
     now rewrite <- IHt1, <- IHt2; firstorder.
@@ -383,8 +220,8 @@ Lemma open_open :
 Proof.
   induction t; cbn; intros * Hneq H.
   - easy.
-  - destruct (PeanoNat.Nat.eqb_spec i n); [| easy].
-    destruct (PeanoNat.Nat.eqb_spec j n); [| easy].
+  - decide (i = n); subst; cbn; [| easy].
+    decide (j = n); [| easy].
     now congruence.
   - inversion H.
     f_equal.
@@ -396,18 +233,9 @@ Proof.
     + now eapply IHt2, H2.
 Qed.
 
-Lemma open_open' :
-  forall (t : Tm) (i : nat) (x : Atom) (u : Tm),
-    t {{ 0 ~> x }} {{ S i ~> u }} = t {{ 0 ~> x }} ->
-      t {{ S i ~> u }} = t.
-Proof.
-  intros.
-  now apply open_open in H.
-Qed.
-
 Inductive lc : Tm -> Prop :=
 | lc_fvar : forall x : Atom, lc x
-| lc_abs  : forall (t : Tm) (l : list Atom), (forall x, ~ In x l -> lc (open' x t)) -> lc (abs t)
+| lc_abs  : forall (t : Tm) (l : list Atom), (forall x, ~ In x l -> lc (t {{ 0 ~> x }})) -> lc (abs t)
 | lc_app  : forall t1 t2 : Tm, lc t1 -> lc t2 -> lc (app t1 t2).
 
 #[export] Hint Constructors lc : core.
@@ -419,8 +247,9 @@ Proof.
   intros t n u Hlc; revert n u.
   induction Hlc; cbn; intros; [easy | |].
   - f_equal.
-    apply open_open' with (fresh l), H0.
-    now apply fresh_spec.
+    eapply open_open; cycle 1.
+    + now apply (H0 (fresh l)), fresh_spec.
+    + easy.
   - now f_equal.
 Qed.
 
@@ -434,7 +263,7 @@ Proof.
   induction t; cbn; intros.
   - rewrite open_lc; [easy |].
     now decide (x = a).
-  - now destruct (PeanoNat.Nat.eqb i n).
+  - now decide (i = n).
   - now rewrite IHt.
   - now rewrite IHt1, IHt2.
 Qed.
@@ -546,7 +375,6 @@ Lemma lc_Typing :
 Proof.
   induction 1; only 1, 3: now constructor.
   apply lc_abs with l.
-  unfold open'.
   intros x Hx.
   now apply H0.
 Qed.
@@ -652,7 +480,7 @@ Lemma open_subst' :
 Proof.
   induction t; cbn; intros i x u Hfresh.
   - now decide (x = a); firstorder congruence.
-  - destruct (PeanoNat.Nat.eqb_spec i n); cbn; [| easy].
+  - decide (i = n); cbn; [| easy].
     now decide (x = x).
   - now erewrite IHt.
   - rewrite in_app_iff in Hfresh.
@@ -792,4 +620,3 @@ Proof.
   specialize (H0 (fresh l) (fresh_spec l)).
   now inversion H0.
 Qed.
-
