LocallyNameless/Atom.v
@@ -1,0 +1,110 @@
+Require Import
+  List
+  Coq.Classes.DecidableClass
+  Lia.
+
+Import ListNotations.
+
+Class isAtom (Atom : Type) : Type :=
+{
+  Decidable_isAtom :: forall x y : Atom, Decidable (x = y);
+  fresh : list Atom -> Atom;
+  fresh_spec : forall l : list Atom, ~ In (fresh l) l;
+}.
+
+Inductive Atom : Type :=
+| Fresh : list Atom -> Atom.
+
+Definition out (x : Atom) : list Atom :=
+match x with
+| Fresh l => l
+end.
+
+(*
+Inductive Atom : Type := Fresh
+{
+  out : list Atom;
+}.
+*)
+
+Fixpoint size (x : Atom) : nat :=
+match x with
+| Fresh l => 1 + fold_right (fun h t => size h + t) 0 l
+end.
+
+Definition sizes l := 1 + fold_right (fun h t => size h + t) 0 l.
+
+Fixpoint eq_dec_Atom (x y : Atom) : {x = y} + {x <> y}.
+Proof.
+  refine
+  (
+    match x, y with
+    | Fresh lx, Fresh ly =>
+      match list_eq_dec eq_dec_Atom lx ly with
+      | left eq => _
+      | right neq => _
+      end
+    end
+  ).
+  - now left; f_equal.
+  - now right; intros [=].
+Defined.
+
+#[export, refine] Instance Decidable_eq_Atom :
+  forall x y : Atom, Decidable (x = y) :=
+{
+  Decidable_witness :=
+    match eq_dec_Atom x y with
+    | left _ => true
+    | right _ => false
+    end;
+}.
+Proof.
+  now destruct (eq_dec_Atom x y).
+Defined.
+
+Lemma In_size :
+  forall (x : Atom) (l : list Atom),
+    In x l -> size x < sizes l.
+Proof.
+  induction l as [| h t IH]; intros Hin; [easy |].
+  destruct Hin as [-> | Hin]; cbn; [now lia |].
+  unfold sizes in IH.
+  specialize (IH Hin).
+  now lia.
+Qed.
+
+#[export, refine] Instance isAtom_Atom : isAtom Atom :=
+{
+  fresh := Fresh;
+}.
+Proof.
+  intros l Hin.
+  apply In_size in Hin. cbn in Hin.
+  now lia.
+Defined.
+
+Fixpoint fresh_nat (l : list nat) : nat :=
+match l with
+| [] => 0
+| h :: t => 1 + max h (fresh_nat t)
+end.
+
+Lemma fresh_nat_aux :
+  forall (l : list nat) (n : nat),
+    In n l -> n < fresh_nat l.
+Proof.
+  induction l as [| h t]; cbn; intros; [easy |].
+  destruct H as [-> | H]; [now lia |].
+  now specialize (IHt _ H); lia.
+Qed.
+
+#[export, refine] Instance isAtom_nat : isAtom nat :=
+{
+  fresh := fresh_nat;
+}.
+Proof.
+  intros l Hin.
+  apply fresh_nat_aux in Hin.
+  now lia.
+Defined.
