LocallyNameless/LocallyNameless.v
@@ -1,0 +1,54 @@
+Require Import
+  Coq.Classes.DecidableClass.
+
+From FormalSystems Require Export LocallyNameless.Atom.
+
+Class OC (Index Atom Term : Type) : Type :=
+{
+  open  : Term -> Index -> Atom -> Term;
+  close : Term -> Index -> Atom -> Term;
+}.
+
+Notation "t {{ i ~> a }}" := (open t i a) (at level 68).
+Notation "t {{ i <~ a }}" := (close t i a) (at level 68).
+
+Class LocallyNameless (Index Atom Term : Type) : Type :=
+{
+  LocallyNameless_isAtom :: isAtom Atom;
+  LocallyNameless_Decidable_eq_Index :: forall i j : Index, Decidable (i = j);
+  LocallyNameless_OC :: OC Index Atom Term;
+  open_open_eq : (* OC 1 *)
+    forall (t : Term) (i : Index) (a b : Atom),
+      t {{ i ~> a }} {{ i ~> b }} = t {{ i ~> a }};
+  close_close_eq : (* OC 2 *)
+    forall (t : Term) (i j : Index) (a : Atom),
+      t {{ i <~ a }} {{ j <~ a }} = t {{ i <~ a }};
+  open_close_eq : (* OC 3 *)
+    forall (t : Term) (i : Index) (a : Atom),
+      t {{ i ~> a }} {{ i <~ a }} = t {{ i <~ a }};
+  close_open_eq : (* OC 4 *)
+    forall (t : Term) (i : Index) (a : Atom),
+      t {{ i <~ a }} {{ i ~> a }} = t {{ i ~> a }};
+  open_open_neq : (* OC 5 *)
+    forall (t : Term) (i j : Index) (a b : Atom),
+      i <> j ->
+        t {{ i ~> a }} {{ j ~> b }} = t {{ j ~> b }} {{ i ~> a }};
+  close_close_neq : (* OC 6 *)
+    forall (t : Term) (i j : Index) (a b : Atom),
+      a <> b ->
+        t {{ i <~ a }} {{ j <~ b }} = t {{ j <~ b }} {{ i <~ a }};
+  open_close_neq : (* OC 7 *)
+    forall (t : Term) (i j : Index) (a b : Atom),
+      i <> j -> a <> b ->
+        t {{ i ~> a }} {{ j <~ b }} = t {{ j <~ b }} {{ i ~> a }};
+  open_close_open : (* OC 8 *)
+    forall (t : Term) (i j : Index) (a b : Atom),
+      t {{ i ~> a }} {{ j <~ a }} {{ j ~> b }}
+        =
+      t {{ j ~> b }} {{ i <~ a }} {{ i ~> b }};
+  close_open_close : (* OC 9 *)
+    forall (t : Term) (i j : Index) (a b : Atom),
+      t {{ i <~ a }} {{ i ~> b }} {{ j <~ b }}
+        =
+      t {{ j <~ b }} {{ i ~> a }} {{ j <~ a }}
+}.
